theories/c_toy_lang/lang_instantiation.v
@@ -74,6 +74,7 @@ Qed.
 Lemma fill_class {p:program} (K : list ectx_item) (e:expr) : 
     is_Some (to_class (ectxi_language.fill K e)) → K = nil ∨ ∃ v, to_class e = Some (ExprVal v).
 Proof.
+  (* TODO use to_val_fill_some *)
   intros [v Hv]. revert v Hv. induction K as [|k1 K] using rev_ind; intros v Hv. 1:now left. right.
   rewrite fill_app in Hv.
   destruct k1; cbn in Hv; try congruence.
@@ -97,6 +98,59 @@ Inductive split_state : state → state → state → Prop :=
 
 Definition fill (K : list ectx_item) (e : expr) : expr :=
   @ectxi_language.fill (C_ectxi_lang (∅ : gmap _ _)) K e.
+
+Lemma fill_comp k K e : fill (k::K) e = fill K (fill_item k e).
+Proof.
+  reflexivity.
+Qed.
+
+Lemma fill_val K e : is_Some (to_val (fill K e)) → is_Some (to_val e).
+Proof.
+  induction K in e|-*.
+  - intros H; apply H.
+  - intros H. cbn in H. specialize (IHK _ H).
+    eapply fill_item_val. apply IHK.
+Qed.
+
+Lemma fill_tail k K e e' : to_val e = None -> to_val e' = None -> fill_item k e = fill K e' -> K = [] ∨ exists K', K = K' ++ [k] /\ e = fill K' e'.
+Proof. intros He He'.
+  destruct K.
+  + intros _. now left.
+  + destruct (@exists_last _ (e0::K)) as (L & l & Hl); first congruence.
+    rewrite Hl. unfold fill, ectxi_language.fill.
+    rewrite foldl_snoc. cbn. intros H. pose proof H as H_copy.
+    apply fill_item_no_val_inj in H_copy as ->.
+    2: easy. 
+    2: { destruct (to_val (foldl (flip fill_item) e' L)) eqn:Heq; last done.
+         edestruct (fill_val L e'). 1: eexists; apply Heq. congruence. }
+    right. eexists. split; first done. now apply fill_item_inj in H.
+Qed.
+
+Lemma fill_ctx K s vv K' e : 
+  fill K' e = fill K (of_class (ExprCall s vv))
+  -> (exists v, e = Val v) \/ (exists K2, e = fill K2 (of_class (ExprCall s vv))).
+Proof. cbn.
+  induction K' as [|[] K' IH] in K,e|-*; try rewrite fill_comp; intros H.
+  2-14: destruct  (IH _ _ H) as [(v & Hv)|(K2 & Hk2)]; try (cbn in *; congruence);
+      try (destruct (to_val e) eqn:Heq; first (apply of_to_val in Heq; by left; eexists);
+           right; pose proof Hk2 as Hk3;
+           apply fill_tail in Hk2 as [->|(K3 & -> & ->)];
+           [ (cbn in Hk3; congruence) |by eexists|(cbn in Hk3; congruence)| done]).
+  + cbn. right. exists K. apply H.
+  + destruct (to_val e) eqn:Heq; first (apply of_to_val in Heq; by left; eexists).
+    right; pose proof Hk2 as Hk3.
+    apply fill_tail in Hk2 as [->|(K3 & -> & ->)];
+    [|by eexists|(cbn in Hk3; congruence)| done].
+    cbn in Hk3. injection Hk3. intros _ ->; cbn in Heq; congruence.
+  + destruct (to_val e) eqn:Heq; first (apply of_to_val in Heq; by left; eexists).
+    right; pose proof Hk2 as Hk3.
+    apply fill_tail in Hk2 as [->|(K3 & -> & ->)];
+    [|by eexists|(cbn in Hk3; congruence)| done].
+    cbn in Hk3. injection Hk3. intros Hc. exfalso.
+    assert (In e (map Val vv)) as (x&<-&_)%in_map_iff.
+    - rewrite -Hc. apply in_or_app. right; now left.
+    - now cbn in Heq.
+Qed.
 
 Lemma melocoton_lang_mixin_C :
   @LanguageMixin expr val function (list ectx_item) state state state
@@ -132,6 +186,7 @@ Proof. split.
     1: econstructor; apply Hstep.
     1: right; destruct Hl as (v&Hv); exists v; destruct e; cbn in *; congruence.
     1: left; now rewrite Hr.
+    
 Qed.
 
 Canonical Structure C_lang_melocoton := Language melocoton_lang_mixin_C.
